Add pipeline example. State transition shallowly gathered.

Examples.v
@@ -1,4 +1,4 @@
-Require Import SGA.Common SGA.Environments SGA.Syntax SGA.Semantics SGA.Types.
+Require Import SGA.Common SGA.Environments SGA.Syntax SGA.Semantics SGA.Types SGA.OneRuleAtATime.
 
 Open Scope bool_scope.
 Require Import Coq.Strings.String.
@@ -17,11 +17,24 @@ Section Functions.
                            | [[a;true]] => vbits [false]
                            | _ => vtt
                            end.
+
+    Definition eq2 arg := match arg with
+                           | [[a;b];[c;d]] =>
+                             vbits [andb (Bool.eqb a c) (Bool.eqb b d)]
+                           | _ => vtt
+                           end.
+
     Definition odd arg := match arg with
                            | [[a;false]] => vbits [false]
                            | [[a;true]] => vbits [true]
                            | _ => vtt
                           end.
+    Definition neg arg := match arg with
+                           | [[false]] => vbits [true]
+                           | [[true]] => vbits [false]
+                           | _ => vtt
+                          end.
+
     Definition threeNPlusOne arg := match arg with (* Fake implementation *)
                              | [[a;b]] => vbits [b;false]
                              | _ => vtt
@@ -36,7 +49,7 @@ End Functions.
 Section Example1.
   Definition r := 0.
   Definition InitReg := putenv env_nil r (cons true (cons false nil)).
-  Inductive Extfuns := Even | Odd | Divide | ThreeNPlusOne | Register (idx: nat).
+  Inductive Extfuns := Eq | Even | Odd | Divide | ThreeNPlusOne | Register  (idx: nat) | Neg | Fabst |Gabst |Streamabst.
 
   Scheme Equality for Extfuns.
   Definition SigmaEnv : Env Extfuns ExternalFunction := EqEnv Extfuns_eq_dec.
@@ -73,17 +86,6 @@ Section Example1.
   Notation "f '[' arg ']'" := (Call f (cons arg nil)) (at level 99,arg at level 99) : sga_scope.
   Notation "f '<|' g" := (Try f%sga g g ) (at level 99, g at level 99, right associativity, only parsing).
 
-  (* Test of notations: *)
-  Check (Let "test" <- Skip in Skip)%sga.
-  Check (Let "used" <- Fail in Var "used")%sga.
-  Check ( Fail; Skip)%sga.
-  Check (r·read_0)%sga.
-  Check (r·write_0(Skip))%sga.
-  Check (Let "used" <- r·read_0 in Var "used")%sga.
-  Check (Even[Skip])%sga.
-  Check (Skip <| Done).
-  Check (Skip <| Fail <| Skip <| Done).
-  Check ((r·read_0) <| Fail <| Skip <| r·write_0(Skip)<| Done).
 
   Definition divide_collatz :=
     (
@@ -218,3 +220,325 @@ Section Example2.
    Compute (interp_rule InitReg sigma env_nil nil nil divide_collatz).
    Compute (interp_rule InitReg sigma env_nil nil nil multiply_collatz).
 End Example2.
+
+
+
+Section Example_Pipeline.
+  Variable f_abst: list bits -> value.
+  Variable g_abst: list bits -> value.
+  Variable stream_abst: list bits -> value.
+  Definition sigma2_abst : (SigmaEnv.(env_t)).
+    refine (putenv _ Fabst {| sig := {| argSizes := cons 2 nil;
+                                        retType := bit_t 2 |};
+                              impl := f_abst|}).
+    refine (putenv _ Streamabst {| sig := {| argSizes := cons 2 nil;
+                                             retType := bit_t 2 |};
+                                   impl := stream_abst |}).
+    refine (putenv _ Neg {| sig := {| argSizes := cons 1 nil;
+                                             retType := bit_t 1 |};
+                            impl := neg |}).
+    refine (putenv _ Eq {| sig := {| argSizes := cons 2 (cons 2 nil);
+                                             retType := bit_t 1 |};
+                                   impl := eq2 |}).
+
+    refine (putenv _ Gabst {| sig := {| argSizes := cons 2 nil;
+                                        retType := bit_t 2 |};
+                              impl := g_abst |}).
+
+    exact env_nil.
+    exact magic.
+    exact magic.
+    exact magic.
+    exact magic.
+    exact magic.
+  Defined.
+
+
+  (* Redefine notations because they conflict with list and I do not know how to handle that properly without Custom_entries *)
+  Delimit Scope sga_scope with sga.
+  Notation "'Let' a '<-' b 'in' c" := (Bind a b c) (at level 99, c at level 98) : sga_scope.
+  Notation " a ';' b " :=  (Bind "nobodynamesavariablelikethat" a b) (at level 10, b at level 100): sga_scope. (* Hack *)
+  Notation "reg '·' 'read_0'" := (Read P0 reg) (at level 10) :sga_scope.
+  Notation "reg '·' 'read_1'" := (Read P1 reg) (at level 10) :sga_scope.
+  Notation "reg '·' 'write_0(' value ')'" := (Write P0 reg value) (at level 10) :sga_scope.
+  Notation "reg '·' 'write_1(' value ')'" := (Write P1 reg value) (at level 10) :sga_scope.
+  Notation "f '[' arg ']'" := (Call f (cons arg nil)) (at level 99,arg at level 99) : sga_scope.
+  Notation "f '[' arg1 ',' arg2 ']'" := (Call f (cons arg1 (cons arg2 nil))) (at level 99,arg1 at level 99, arg2 at level 99) : sga_scope.
+  Notation "f '<|' g" := (Try f%sga g g ) (at level 99, g at level 99, right associativity, only parsing).
+
+  (* Test of notations: *)
+  Check (Let "test" <- Skip in Skip)%sga.
+  Check (Let "used" <- Fail in Var "used" ; Skip)%sga.
+  Check ( Fail; Skip)%sga.
+  Check (r·read_0)%sga.
+  Check (r·write_0(Skip))%sga.
+  Check (Let "used" <- r·read_0 in Var "used")%sga.
+  Check (Even[Skip])%sga.
+  Check (Skip <| Done).
+  Check (Skip <| Fail <| Skip <| Done).
+  Check ((r·read_0) <| Fail <| Skip <| r·write_0(Skip)<| Done).
+  Check collatz.
+  (* Manually we step through destructs to learn that those are the hypthesis that we need to reduce the computation *)
+
+
+  Definition outputReg := 2.
+  Definition inputReg := 1.
+  Definition invalid := 3.
+  Definition correct:= 4.
+
+  Definition  doF:=
+    (Let "v" <- inputReg·read_0 in
+     inputReg·write_0(Streamabst[Var"v"]);
+     Let "invalid" <- invalid·read_1 in
+     If (Var"invalid")
+        (invalid·write_1(Const (cons false nil));
+        r·write_0(Fabst[Var"v"]))
+        Fail
+    )%sga.
+
+  Definition doG :=
+    (
+      Let "invalid" <- invalid·read_0 in
+      If (Neg[Var"invalid"])
+         (
+           Let "data" <- r·read_0 in
+           Let "v" <- outputReg·read_0 in
+           (outputReg·write_0(Streamabst[Var"v"]));
+           invalid·write_0(Const (cons true nil));
+           If (Eq[Gabst[Var"data"],Gabst[Fabst[Var"v"]]])
+              (Skip)
+              (correct·write_0(Const (cons false nil)))
+         )
+         Fail
+    )%sga.
+
+  Definition Pipeline :=  doG <| doF <| Done.
+
+
+  Variable r0 r1 d0 d1 inv : bool.
+  Definition InitReg_1 := putenv (putenv (putenv (putenv (putenv env_nil correct (cons true nil)) invalid (cons inv nil)) inputReg (cons r1 (cons r0 nil))) outputReg (cons r1 (cons r0 nil))) r (cons d0 (cons d1 nil)).
+
+  Variable AF :  (forall r1 r0, { v01 & f_abst ((r1 :: r0 :: nil) :: nil)= vbits (cons (fst v01) (cons (snd v01) nil))}) .
+
+  Variable AG :  (forall r1 r0, { v01 & g_abst ((r1 :: r0 :: nil) :: nil)= vbits (cons (fst v01) (cons (snd v01) nil))}) .
+  Variable AStream :  (forall r1 r0, { v01 & stream_abst ((r1 :: r0 :: nil) :: nil)= vbits (cons (fst v01) (cons (snd v01) nil))}) .
+
+  
+   Lemma caract_pipeline : {t & (interp_scheduler
+           InitReg_1
+           sigma2_abst
+           nil
+           Pipeline) = t}.
+     cbn.
+     eexists.
+     instantiate (1:=ltac:(destruct inv)); destruct inv.
+     cbn.
+     rewrite (projT2 (AStream r1 r0)).
+     cbn.
+     rewrite (projT2 (AF _ _)).
+     cbn.
+     reflexivity.
+     setoid_rewrite (projT2 (AStream r1 r0)).
+     cbn.
+     setoid_rewrite (projT2 (AG d0 d1)).
+     cbn.
+     rewrite (projT2 (AF r1 r0)).
+     cbn.
+     setoid_rewrite (projT2 (AG (fst (projT1 (AF r1 r0)))(snd (projT1 (AF r1 r0))))).
+     cbn.
+     instantiate (1:=ltac:( destruct (Bool.eqb (fst (projT1 (AG (fst (projT1 (AF r1 r0))) (snd (projT1 (AF r1 r0))))))
+        (fst (projT1 (AG d0 d1))) &&
+      Bool.eqb (snd (projT1 (AG (fst (projT1 (AF r1 r0))) (snd (projT1 (AF r1 r0))))))
+      (snd (projT1 (AG d0 d1))))));     destruct (Bool.eqb (fst (projT1 (AG (fst (projT1 (AF r1 r0))) (snd (projT1 (AF r1 r0))))))
+        (fst (projT1 (AG d0 d1))) &&
+      Bool.eqb (snd (projT1 (AG (fst (projT1 (AF r1 r0))) (snd (projT1 (AF r1 r0))))))
+      (snd (projT1 (AG d0 d1)))).
+     -
+     cbn.
+     setoid_rewrite (projT2 (AStream r1 r0)).
+     cbn.
+     rewrite (projT2 (AF r1 r0)).
+     cbn.
+     reflexivity.
+     -
+       cbn.
+       setoid_rewrite (projT2 (AStream r1 r0)).
+       cbn.
+       rewrite (projT2 (AF r1 r0)).
+       cbn.
+       reflexivity.
+   Defined.
+   Eval cbn in (projT1 caract_pipeline).
+
+   Lemma caract_pipeline_update : {t & (interp_scheduler_trace_and_update
+           InitReg_1
+           sigma2_abst
+           nil
+           Pipeline) = t}.
+     unfold interp_scheduler_trace_and_update.
+     cbn.
+     eexists.
+     instantiate (1:=ltac:(destruct inv)); destruct inv.
+     cbn.
+     rewrite (projT2 (AStream r1 r0)).
+     cbn.
+     rewrite (projT2 (AF _ _)).
+     cbn.
+     reflexivity.
+     setoid_rewrite (projT2 (AStream r1 r0)).
+     cbn.
+     setoid_rewrite (projT2 (AG d0 d1)).
+     cbn.
+     rewrite (projT2 (AF r1 r0)).
+     cbn.
+     setoid_rewrite (projT2 (AG (fst (projT1 (AF r1 r0)))(snd (projT1 (AF r1 r0))))).
+     cbn.
+     instantiate (1:=ltac:( destruct (Bool.eqb (fst (projT1 (AG (fst (projT1 (AF r1 r0))) (snd (projT1 (AF r1 r0))))))
+        (fst (projT1 (AG d0 d1))) &&
+      Bool.eqb (snd (projT1 (AG (fst (projT1 (AF r1 r0))) (snd (projT1 (AF r1 r0))))))
+      (snd (projT1 (AG d0 d1))))));     destruct (Bool.eqb (fst (projT1 (AG (fst (projT1 (AF r1 r0))) (snd (projT1 (AF r1 r0))))))
+        (fst (projT1 (AG d0 d1))) &&
+      Bool.eqb (snd (projT1 (AG (fst (projT1 (AF r1 r0))) (snd (projT1 (AF r1 r0))))))
+      (snd (projT1 (AG d0 d1)))).
+     -
+     cbn.
+     setoid_rewrite (projT2 (AStream r1 r0)).
+     cbn.
+     rewrite (projT2 (AF r1 r0)).
+     cbn.
+     reflexivity.
+     -
+       cbn.
+       setoid_rewrite (projT2 (AStream r1 r0)).
+       cbn.
+       rewrite (projT2 (AF r1 r0)).
+       cbn.
+       reflexivity.
+   Defined.
+   Eval cbn in  (projT1 caract_pipeline_update).
+   (* So we need to prove that starting from $v$ = false, we will never reach a case where  *)
+   (* From that we get that the condition for the two rules to fire simultaneously is $v$ *)
+(*       We also get that the condition for the correctness is *)
+
+(*        not v ->   Bool.eqb (fst (projT1 (AG (fst (projT1 (AF r1 r0))) (snd (projT1 (AF r1 r0)))))) *)
+(*            (fst (projT1 (AG d0 d1))) && *)
+(*          Bool.eqb (snd (projT1 (AG (fst (projT1 (AF r1 r0))) (snd (projT1 (AF r1 r0)))))) *)
+(*            (snd (projT1 (AG d0 d1))). *)
+
+   (* We end up having to prove that v is kept the rest of the time *)
+   (* Indeed we end up with
+         Bool.eqb (fst (projT1 (AG (fst (projT1 (AF r1 r0))) (snd (projT1 (AF r1 r0))))))
+           (fst (projT1 (AG d0 d1))) &&
+         Bool.eqb (snd (projT1 (AG (fst (projT1 (AF r1 r0))) (snd (projT1 (AF r1 r0))))))
+           (snd (projT1 (AG d0 d1)))
+ *)
+
+
+   Compute (interp_rule InitReg sigma env_nil nil nil divide_collatz).
+   Compute (interp_rule InitReg sigma env_nil nil nil multiply_collatz).
+End Example2.
+
+
+
+  Variable r0 r1 d0 d1 v c: bool.
+  Definition InitReg_1 := putenv (putenv (putenv (putenv (putenv env_nil correct (cons c nil)) invalid (cons true nil)) inputReg (cons r1 (cons r0 nil))) outputReg (cons r1 (cons r0 nil))) r (cons d0 (cons d1 nil)).
+
+  Variable AF :  (forall r1 r0, { v01 & f_abst ((r1 :: r0 :: nil) :: nil)= vbits (cons (fst v01) (cons (snd v01) nil))}) .
+
+  Variable AG :  (forall r1 r0, { v01 & g_abst ((r1 :: r0 :: nil) :: nil)= vbits (cons (fst v01) (cons (snd v01) nil))}) .
+  Variable AStream :  (forall r1 r0, { v01 & stream_abst ((r1 :: r0 :: nil) :: nil)= vbits (cons (fst v01) (cons (snd v01) nil))}) .
+  (* Note that we do not need the relationship between Odd and Even at that level *)
+  (* And nothing about Div *)
+
+   Lemma caract_pipeline : {t & (interp_scheduler
+           InitReg_1
+           sigma2_abst
+           nil
+           Pipeline) = t}.
+     cbn.
+     eexists.
+     instantiate (1:=ltac:(destruct v)); destruct v.
+     cbn.
+     rewrite (projT2 (AStream r1 r0)).
+     cbn.
+     rewrite (projT2 (AF _ _)).
+     cbn.
+     reflexivity.
+     setoid_rewrite (projT2 (AStream r1 r0)).
+     cbn.
+     setoid_rewrite (projT2 (AG d0 d1)).
+     cbn.
+     rewrite (projT2 (AF r1 r0)).
+     cbn.
+     setoid_rewrite (projT2 (AG (fst (projT1 (AF r1 r0)))(snd (projT1 (AF r1 r0))))).
+     cbn.
+     instantiate (1:=ltac:( destruct (Bool.eqb (fst (projT1 (AG (fst (projT1 (AF r1 r0))) (snd (projT1 (AF r1 r0))))))
+        (fst (projT1 (AG d0 d1))) &&
+      Bool.eqb (snd (projT1 (AG (fst (projT1 (AF r1 r0))) (snd (projT1 (AF r1 r0))))))
+      (snd (projT1 (AG d0 d1))))));     destruct (Bool.eqb (fst (projT1 (AG (fst (projT1 (AF r1 r0))) (snd (projT1 (AF r1 r0))))))
+        (fst (projT1 (AG d0 d1))) &&
+      Bool.eqb (snd (projT1 (AG (fst (projT1 (AF r1 r0))) (snd (projT1 (AF r1 r0))))))
+      (snd (projT1 (AG d0 d1)))).
+     -
+     cbn.
+     setoid_rewrite (projT2 (AStream r1 r0)).
+     cbn.
+     rewrite (projT2 (AF r1 r0)).
+     cbn.
+     reflexivity.
+     -
+       cbn.
+       setoid_rewrite (projT2 (AStream r1 r0)).
+       cbn.
+       rewrite (projT2 (AF r1 r0)).
+       cbn.
+       reflexivity.
+   Defined.
+   Eval cbn in (projT1 caract_pipeline).
+
+   Lemma caract_pipeline_update : {t & (interp_scheduler_trace_and_update
+           InitReg_1
+           sigma2_abst
+           nil
+           Pipeline) = t}.
+     unfold interp_scheduler_trace_and_update.
+     cbn.
+     eexists.
+     instantiate (1:=ltac:(destruct v)); destruct v.
+     cbn.
+     rewrite (projT2 (AStream r1 r0)).
+     cbn.
+     rewrite (projT2 (AF _ _)).
+     cbn.
+     reflexivity.
+     setoid_rewrite (projT2 (AStream r1 r0)).
+     cbn.
+     setoid_rewrite (projT2 (AG d0 d1)).
+     cbn.
+     rewrite (projT2 (AF r1 r0)).
+     cbn.
+     setoid_rewrite (projT2 (AG (fst (projT1 (AF r1 r0)))(snd (projT1 (AF r1 r0))))).
+     cbn.
+     instantiate (1:=ltac:( destruct (Bool.eqb (fst (projT1 (AG (fst (projT1 (AF r1 r0))) (snd (projT1 (AF r1 r0))))))
+        (fst (projT1 (AG d0 d1))) &&
+      Bool.eqb (snd (projT1 (AG (fst (projT1 (AF r1 r0))) (snd (projT1 (AF r1 r0))))))
+      (snd (projT1 (AG d0 d1))))));     destruct (Bool.eqb (fst (projT1 (AG (fst (projT1 (AF r1 r0))) (snd (projT1 (AF r1 r0))))))
+        (fst (projT1 (AG d0 d1))) &&
+      Bool.eqb (snd (projT1 (AG (fst (projT1 (AF r1 r0))) (snd (projT1 (AF r1 r0))))))
+      (snd (projT1 (AG d0 d1)))).
+     -
+     cbn.
+     setoid_rewrite (projT2 (AStream r1 r0)).
+     cbn.
+     rewrite (projT2 (AF r1 r0)).
+     cbn.
+     reflexivity.
+     -
+       cbn.
+       setoid_rewrite (projT2 (AStream r1 r0)).
+       cbn.
+       rewrite (projT2 (AF r1 r0)).
+       cbn.
+       reflexivity.
+   Defined.
+   Eval cbn in  (projT1 caract_pipeline_update).
